src/opt/Simulation.v
@@ -16,66 +16,72 @@ Require Import MemInv.
 Set Implicit Arguments.
 
 
-Section SimulationThread.
+Section SimulationLocal.
   Variable (lang_src lang_tgt:Language.t).
 
   Definition SIM_TERMINAL :=
     forall (st_src:lang_src.(Language.state)) (st_tgt:lang_tgt.(Language.state)), Prop.
 
+  Definition SIM_LOCAL := forall (th_src th_tgt:Local.t), Prop.
+
+  Inductive sim_local (th_src th_tgt:Local.t): Prop :=
+  | sim_local_intro
+      (COMMIT: Commit.le th_src.(Local.commit) th_tgt.(Local.commit))
+      (PROMISE: MemInv.sem Memory.bot th_src.(Local.promise) th_tgt.(Local.promise))
+  .
+
   Definition SIM_THREAD :=
     forall (sim_terminal: SIM_TERMINAL)
-      (st1_src:lang_src.(Language.state)) (th1_src:Thread.t) (mem_k_src:Memory.t)
-      (st1_tgt:lang_tgt.(Language.state)) (th1_tgt:Thread.t) (mem_k_tgt:Memory.t), Prop.
+      (st1_src:lang_src.(Language.state)) (th1_src:Local.t) (mem_k_src:Memory.t)
+      (st1_tgt:lang_tgt.(Language.state)) (th1_tgt:Local.t) (mem_k_tgt:Memory.t), Prop.
 
   (* TODO: inftau & liveness *)
   Definition _sim_thread
              (sim_thread: SIM_THREAD)
              (sim_terminal: SIM_TERMINAL)
-             (st1_src:lang_src.(Language.state)) (th1_src:Thread.t) (mem_k_src:Memory.t)
-             (st1_tgt:lang_tgt.(Language.state)) (th1_tgt:Thread.t) (mem_k_tgt:Memory.t): Prop :=
+             (st1_src:lang_src.(Language.state)) (th1_src:Local.t) (mem_k_src:Memory.t)
+             (st1_tgt:lang_tgt.(Language.state)) (th1_tgt:Local.t) (mem_k_tgt:Memory.t): Prop :=
     forall mem1_src mem1_tgt
       (MEMORY: sim_memory mem1_src mem1_tgt)
       (FUTURE_SRC: Memory.future mem_k_src mem1_src)
       (FUTURE_TGT: Memory.future mem_k_tgt mem1_tgt)
-      (WF_SRC: Thread.wf th1_src mem1_src)
-      (WF_TGT: Thread.wf th1_tgt mem1_tgt),
+      (WF_SRC: Local.wf th1_src mem1_src)
+      (WF_TGT: Local.wf th1_tgt mem1_tgt),
       <<TERMINAL:
         forall (TERMINAL_TGT: lang_tgt.(Language.is_terminal) st1_tgt),
         exists st2_src th2_src mem2_src,
-          <<STEPS: rtc (@Executor.internal_step lang_src)
-                       (Executor.mk _ st1_src th1_src mem1_src)
-                       (Executor.mk _ st2_src th2_src mem2_src)>> /\
+          <<STEPS: rtc (@Thread.internal_step lang_src)
+                       (Thread.mk _ st1_src th1_src mem1_src)
+                       (Thread.mk _ st2_src th2_src mem2_src)>> /\
           <<MEMORY: sim_memory mem2_src mem1_tgt>> /\
           <<TERMINAL_SRC: lang_src.(Language.is_terminal) st2_src>> /\
-          <<COMMIT: Commit.le th2_src.(Thread.commit) th1_tgt.(Thread.commit)>> /\
-          <<PROMISE: MemInv.sem Memory.bot th2_src.(Thread.promise) th1_tgt.(Thread.promise)>> /\
-          <<SIM: sim_terminal st2_src st1_tgt>>>> /\
+          <<LOCAL: sim_local th2_src th1_tgt>> /\
+          <<TERMINAL: sim_terminal st2_src st1_tgt>>>> /\
       <<FUTURE:
         forall mem2_src
           (FUTURE_SRC: Memory.future mem1_src mem2_src)
-          (WF_SRC: Thread.wf th1_src mem2_src),
+          (WF_SRC: Local.wf th1_src mem2_src),
         exists mem2_tgt,
           <<MEMORY: sim_memory mem2_src mem2_tgt>> /\
           <<FUTURE_TGT: Memory.future mem1_tgt mem2_tgt>> /\
-          <<WF_TGT: Thread.wf th1_tgt mem2_tgt>>>> /\
+          <<WF_TGT: Local.wf th1_tgt mem2_tgt>>>> /\
       <<PROMISE:
-        forall (PROMISE_TGT: th1_tgt.(Thread.promise) = Memory.bot),
+        forall (PROMISE_TGT: th1_tgt.(Local.promise) = Memory.bot),
         exists st2_src th2_src mem2_src,
-          <<STEPS: rtc (@Executor.internal_step lang_src)
-                       (Executor.mk _ st1_src th1_src mem1_src)
-                       (Executor.mk _ st2_src th2_src mem2_src)>> /\
-          <<MEMORY: sim_memory mem2_src mem1_tgt>> /\
-          <<PROMISE_SRC: th2_src.(Thread.promise) = Memory.bot>>>> /\
+          <<STEPS: rtc (@Thread.internal_step lang_src)
+                       (Thread.mk _ st1_src th1_src mem1_src)
+                       (Thread.mk _ st2_src th2_src mem2_src)>> /\
+          <<PROMISE_SRC: th2_src.(Local.promise) = Memory.bot>>>> /\
       <<STEP:
         forall e st3_tgt th3_tgt mem3_tgt
-          (STEP_TGT: Executor.step (Executor.mk _ st1_tgt th1_tgt mem1_tgt) e
-                                   (Executor.mk _ st3_tgt th3_tgt mem3_tgt)),
+          (STEP_TGT: Thread.step (Thread.mk _ st1_tgt th1_tgt mem1_tgt) e
+                                   (Thread.mk _ st3_tgt th3_tgt mem3_tgt)),
         exists st2_src th2_src mem2_src st3_src th3_src mem3_src,
-          <<STEPS: rtc (@Executor.internal_step lang_src)
-                       (Executor.mk _ st1_src th1_src mem1_src)
-                       (Executor.mk _ st2_src th2_src mem2_src)>> /\
-          <<STEP_SRC: Executor.step (Executor.mk _ st2_src th2_src mem2_src) e
-                                    (Executor.mk _ st3_src th3_src mem3_src)>> /\
+          <<STEPS: rtc (@Thread.internal_step lang_src)
+                       (Thread.mk _ st1_src th1_src mem1_src)
+                       (Thread.mk _ st2_src th2_src mem2_src)>> /\
+          <<STEP_SRC: Thread.step (Thread.mk _ st2_src th2_src mem2_src) e
+                                    (Thread.mk _ st3_src th3_src mem3_src)>> /\
           <<MEMORY2: sim_memory mem3_src mem3_tgt>> /\
           <<SIM: sim_thread sim_terminal st3_src th3_src mem3_src st3_tgt th3_tgt mem3_tgt>>>>.
 
@@ -103,14 +109,14 @@ Section SimulationThread.
     - i. exploit STEP; eauto. i. des; [|done].
       eexists _, _, _, _, _, _. splits; eauto.
   Qed.
-End SimulationThread.
+End SimulationLocal.
 Hint Resolve _sim_thread_mon: paco.
 
 
 Section Simulation.
   Definition SIM :=
-    forall (th1_src:Threads.t) (mem_k_src:Memory.t)
-      (th1_tgt:Threads.t) (mem_k_tgt:Memory.t), Prop.
+    forall (ths1_src:Threads.t) (mem_k_src:Memory.t)
+      (ths1_tgt:Threads.t) (mem_k_tgt:Memory.t), Prop.
 
   (* TODO: inftau & liveness *)
   Definition _sim
@@ -186,8 +192,8 @@ Qed.
 Lemma singleton_consistent
       tid lang st th mem:
   Configuration.consistent (Configuration.mk (IdentMap.singleton tid (existT _ _ st, th)) mem) <->
-  <<WF: Thread.wf th mem>> /\
-  <<CONSISTENT: Executor.consistent lang st th mem>>.
+  <<WF: Local.wf th mem>> /\
+  <<CONSISTENT: Thread.consistent lang st th mem>>.
 Proof.
   econs; intro X.
   - inv X. ss.
@@ -206,7 +212,7 @@ Lemma singleton_is_terminal
       tid lang st th:
   Threads.is_terminal (IdentMap.singleton tid (existT _ _ st, th)) <->
   <<STATE: lang.(Language.is_terminal) st>> /\
-  <<THREAD: Thread.is_terminal th>>.
+  <<THREAD: Local.is_terminal th>>.
 Proof.
   econs; intro X.
   - eapply X. apply IdentMap.singleton_find.
@@ -221,29 +227,29 @@ Lemma sim_step
       st1_src th1_src mem1_src
       st1_tgt th1_tgt mem1_tgt
       st3_tgt th3_tgt mem3_tgt
-      (STEP: @Executor.step lang_tgt
-                            (Executor.mk _ st1_tgt th1_tgt mem1_tgt) e
-                            (Executor.mk _ st3_tgt th3_tgt mem3_tgt))
+      (STEP: @Thread.step lang_tgt
+                            (Thread.mk _ st1_tgt th1_tgt mem1_tgt) e
+                            (Thread.mk _ st3_tgt th3_tgt mem3_tgt))
       (MEMORY: sim_memory mem1_src mem1_tgt)
-      (WF_SRC: Thread.wf th1_src mem1_src)
-      (WF_TGT: Thread.wf th1_tgt mem1_tgt)
+      (WF_SRC: Local.wf th1_src mem1_src)
+      (WF_TGT: Local.wf th1_tgt mem1_tgt)
       (SIM: sim_thread sim_terminal st1_src th1_src mem1_src st1_tgt th1_tgt mem1_tgt):
   exists st2_src th2_src mem2_src st3_src th3_src mem3_src,
-    <<STEPS: rtc (@Executor.internal_step lang_src)
-                 (Executor.mk _ st1_src th1_src mem1_src)
-                 (Executor.mk _ st2_src th2_src mem2_src)>> /\
-    <<STEP: Executor.step (Executor.mk _ st2_src th2_src mem2_src) e
-                          (Executor.mk _ st3_src th3_src mem3_src)>> /\
+    <<STEPS: rtc (@Thread.internal_step lang_src)
+                 (Thread.mk _ st1_src th1_src mem1_src)
+                 (Thread.mk _ st2_src th2_src mem2_src)>> /\
+    <<STEP: Thread.step (Thread.mk _ st2_src th2_src mem2_src) e
+                          (Thread.mk _ st3_src th3_src mem3_src)>> /\
     <<MEMORY: sim_memory mem3_src mem3_tgt>> /\
-    <<WF_SRC: Thread.wf th3_src mem3_src>> /\
-    <<WF_TGT: Thread.wf th3_tgt mem3_tgt>> /\
+    <<WF_SRC: Local.wf th3_src mem3_src>> /\
+    <<WF_TGT: Local.wf th3_tgt mem3_tgt>> /\
     <<SIM: sim_thread sim_terminal st3_src th3_src mem3_src st3_tgt th3_tgt mem3_tgt>>.
 Proof.
-  exploit Executor.step_future; eauto. s. i. des.
+  exploit Thread.step_future; eauto. s. i. des.
   punfold SIM. exploit SIM; eauto; try reflexivity. i. des.
   exploit STEP0; eauto. i. des; [|done].
-  exploit Executor.rtc_internal_step_future; eauto. s. i. des.
-  exploit Executor.step_future; eauto. s. i. des.
+  exploit Thread.rtc_internal_step_future; eauto. s. i. des.
+  exploit Thread.step_future; eauto. s. i. des.
   eexists _, _, _, _, _, _. splits; eauto.
 Qed.
 
@@ -252,19 +258,19 @@ Lemma sim_rtc_internal_step
       sim_terminal
       st1_src th1_src mem1_src
       e1_tgt e2_tgt
-      (STEPS: rtc (@Executor.internal_step lang_tgt) e1_tgt e2_tgt)
-      (MEMORY: sim_memory mem1_src e1_tgt.(Executor.memory))
-      (WF_SRC: Thread.wf th1_src mem1_src)
-      (WF_TGT: Thread.wf e1_tgt.(Executor.thread) e1_tgt.(Executor.memory))
-      (SIM: sim_thread sim_terminal st1_src th1_src mem1_src e1_tgt.(Executor.state) e1_tgt.(Executor.thread) e1_tgt.(Executor.memory)):
+      (STEPS: rtc (@Thread.internal_step lang_tgt) e1_tgt e2_tgt)
+      (MEMORY: sim_memory mem1_src e1_tgt.(Thread.memory))
+      (WF_SRC: Local.wf th1_src mem1_src)
+      (WF_TGT: Local.wf e1_tgt.(Thread.thread) e1_tgt.(Thread.memory))
+      (SIM: sim_thread sim_terminal st1_src th1_src mem1_src e1_tgt.(Thread.state) e1_tgt.(Thread.thread) e1_tgt.(Thread.memory)):
   exists st2_src th2_src mem2_src,
-    <<STEPS: rtc (@Executor.internal_step lang_src)
-                 (Executor.mk _ st1_src th1_src mem1_src)
-                 (Executor.mk _ st2_src th2_src mem2_src)>> /\
-    <<MEMORY: sim_memory mem2_src e2_tgt.(Executor.memory)>> /\
-    <<WF_SRC: Thread.wf th2_src mem2_src>> /\
-    <<WF_TGT: Thread.wf e2_tgt.(Executor.thread) e2_tgt.(Executor.memory)>> /\
-    <<SIM: sim_thread sim_terminal st2_src th2_src mem2_src e2_tgt.(Executor.state) e2_tgt.(Executor.thread) e2_tgt.(Executor.memory)>>.
+    <<STEPS: rtc (@Thread.internal_step lang_src)
+                 (Thread.mk _ st1_src th1_src mem1_src)
+                 (Thread.mk _ st2_src th2_src mem2_src)>> /\
+    <<MEMORY: sim_memory mem2_src e2_tgt.(Thread.memory)>> /\
+    <<WF_SRC: Local.wf th2_src mem2_src>> /\
+    <<WF_TGT: Local.wf e2_tgt.(Thread.thread) e2_tgt.(Thread.memory)>> /\
+    <<SIM: sim_thread sim_terminal st2_src th2_src mem2_src e2_tgt.(Thread.state) e2_tgt.(Thread.thread) e2_tgt.(Thread.memory)>>.
 Proof.
   revert st1_src th1_src mem1_src MEMORY WF_SRC WF_TGT SIM.
   induction STEPS; i.
@@ -287,10 +293,10 @@ Lemma sim_thread_consistent
       st_tgt th_tgt mem_tgt
       (SIM: sim_thread sim_terminal st_src th_src mem_src st_tgt th_tgt mem_tgt)
       (MEMORY: sim_memory mem_src mem_tgt)
-      (WF_SRC: Thread.wf th_src mem_src)
-      (WF_TGT: Thread.wf th_tgt mem_tgt)
-      (CONSISTENT: Executor.consistent lang_tgt st_tgt th_tgt mem_tgt):
-  Executor.consistent lang_src st_src th_src mem_src.
+      (WF_SRC: Local.wf th_src mem_src)
+      (WF_TGT: Local.wf th_tgt mem_tgt)
+      (CONSISTENT: Thread.consistent lang_tgt st_tgt th_tgt mem_tgt):
+  Thread.consistent lang_src st_src th_src mem_src.
 Proof.
   generalize SIM. intro X.
   punfold X. exploit X; eauto; try reflexivity. i. des.
@@ -301,7 +307,7 @@ Proof.
   i. des. destruct e2. ss.
   punfold SIM0. exploit SIM0; eauto; try reflexivity. i. des.
   exploit PROMISE1; eauto. i. des.
-  eexists (Executor.mk _ _ _ _). splits; [|eauto].
+  eexists (Thread.mk _ _ _ _). splits; [|eauto].
   etransitivity; eauto.
 Qed.
 
@@ -333,14 +339,14 @@ Proof.
         { eapply IdentMap.singleton_find. }
         { econs 1. eauto. }
         { ii. eexists. splits; eauto. ss.
-          apply MemInv.sem_bot_inv in PROMISE0. etransitivity; eauto.
+          inv LOCAL. apply MemInv.sem_bot_inv in PROMISE0. etransitivity; eauto.
           apply THREAD.
         }
       * inv X. s. erewrite IdentMap.singleton_add. econs.
     + ii. ss. rewrite IdentMap.singleton_add in *.
       apply IdentMap.singleton_find_inv in FIND. des. subst.
       splits; Configuration.simplify. econs; eauto.
-      apply MemInv.sem_bot_inv in PROMISE0. etransitivity; eauto.
+      inv LOCAL. apply MemInv.sem_bot_inv in PROMISE0. etransitivity; eauto.
       apply THREAD.
   - i. inv STEP_TGT. ss.
     apply IdentMap.singleton_find_inv in TID. des.
