src/while/Syntax.v
@@ -78,45 +78,54 @@ Module Instr.
     | expr_op2 _ op1 op2 => RegSet.union (Value.regs_of op1) (Value.regs_of op2)
     end.
 
+  Inductive rmw :=
+  | fetch_add (addendum:Value.t)
+  | cas (old new:Value.t)
+  .
+
   Inductive t :=
-  | nop
   | assign (lhs:Reg.t) (rhs:expr)
   | load (lhs:Reg.t) (rhs:Loc.t) (ord:Ordering.t)
   | store (lhs:Loc.t) (rhs:Value.t) (ord:Ordering.t)
-  | fetch_add (lhs:Reg.t) (loc:Loc.t) (addendum:Value.t) (ord:Ordering.t)
+  | update (lhs:Reg.t) (loc:Loc.t) (rmw:rmw) (ord:Ordering.t)
   | fence (ord:Ordering.t)
   | syscall (lhs:Reg.t) (rhses:list Value.t)
   .
 
+  Definition skip := fence Ordering.relaxed.
+
   Definition ordering_of (i:t): Ordering.t :=
     match i with
-    | nop => Ordering.relaxed
     | assign _ _ => Ordering.relaxed
     | load _ _ ord => ord
     | store _ _ ord => ord
-    | fetch_add _ _ _ ord => ord
+    | update _ _ _ ord => ord
     | fence ord => ord
     | syscall _ _ => Ordering.relaxed
     end.
 
   Definition loc_of (i:t): option Loc.t :=
     match i with
-    | nop => None
     | assign _ _ => None
     | load _ loc _ => Some loc
     | store loc _ _ => Some loc
-    | fetch_add _ loc _ _ => Some loc
+    | update _ loc _ _ => Some loc
     | fence _ => None
     | syscall _ _ => None
     end.
 
+  Definition regs_of_rmw (rmw:rmw): RegSet.t :=
+    match rmw with
+    | fetch_add addendum => (Value.regs_of addendum)
+    | cas old new => RegSet.union (Value.regs_of old) (Value.regs_of new)
+    end.
+
   Definition regs_of (i:t): RegSet.t :=
     match i with
-    | nop => RegSet.empty
     | assign reg rhs => RegSet.add reg (regs_of_expr rhs)
     | load reg _ _ => RegSet.singleton reg
     | store _ val _ => Value.regs_of val
-    | fetch_add reg _ val _ => RegSet.add reg (Value.regs_of val)
+    | update reg _ rmw _ => RegSet.add reg (regs_of_rmw rmw)
     | fence _ => RegSet.empty
     | syscall lhs rhses => RegSet.add lhs (Value.regs_of_list rhses)
     end.
@@ -151,11 +160,12 @@ Module SyntaxNotations.
   Notation "e1 'SUB' e2" := (Instr.expr_op2 Op2.sub e2 e2) (at level 41).
   Notation "e1 'MUL' e2" := (Instr.expr_op2 Op2.mul e2 e2) (at level 41).
 
-  Notation "'NOP'" := (Instr.nop) (at level 42).
+  Notation "'SKIP'" := (Instr.skip) (at level 42).
   Notation "'LET' lhs '::=' rhs" := (Instr.assign lhs rhs) (at level 42).
   Notation "'LOAD' lhs '::=' rhs '@' ord" := (Instr.load lhs rhs ord) (at level 42).
   Notation "'STORE' lhs '::=' rhs '@' ord" := (Instr.store lhs rhs ord) (at level 42).
-  Notation "'FETCH_ADD' lhs '::=' loc ',' addendum '@' ord" := (Instr.fetch_add lhs loc addendum ord) (at level 42).
+  Notation "'FETCH_ADD' lhs '::=' loc ',' addendum '@' ord" := (Instr.update lhs loc (Instr.fetch_add addendum) ord) (at level 42).
+  Notation "'CAS' lhs '::=' loc ',' old ',' new '@' ord" := (Instr.update lhs loc (Instr.cas old new) ord) (at level 42).
   Notation "'FENCE' '@' ord" := (Instr.fence ord) (at level 42).
   Notation "'SYSCALL' lhs '::=' rhses" := (Instr.syscall lhs rhses) (at level 42).
 
@@ -164,7 +174,7 @@ Module SyntaxNotations.
 
   Program Definition example1: list Stmt.t := [
     DO [
-      NOP;
+      SKIP;
       LOAD %r"r1" ::= %l"flag" @ acq;
       LET %r"r2" ::= NOT %r"r1"
     ] WHILE (%r"r2" ADD 0);
@@ -173,12 +183,17 @@ Module SyntaxNotations.
 
   Program Definition example2: list Stmt.t := [
     DO [
-      NOP;
+      SKIP;
       LOAD %r"r1" ::= %l"flag" @ rlx;
       LET %r"r2" ::= NOT %r"r1"
     ] WHILE (%r"r2" MUL 1);
     FENCE @ acq;
     LOAD %r"r3" ::= %l"x" @ rlx;
     SYSCALL %r"r4" ::= [%r"r3"; 3; 4]
+  ].
+
+  Program Definition example3: list Stmt.t := [
+    FETCH_ADD %r"r1" ::= %l"x", 1 @ rlx;
+    CAS %r"r1" ::= %l"x", 1, 2 @ rlx
   ].
 End SyntaxNotations.
