src/opt/Composition.v
@@ -33,15 +33,15 @@ Section Compose.
   Qed.
 
   Lemma compose_forall P:
-    (forall tid lang st th (TH: IdentMap.find tid (Threads.compose ths1 ths2) = Some (existT _ lang st, th)),
-        (P tid lang th):Prop) <->
-    (forall tid lang st th (TH: IdentMap.find tid ths1 = Some (existT _ lang st, th)),
-        (P tid lang th):Prop) /\
-    (forall tid lang st th (TH: IdentMap.find tid ths2 = Some (existT _ lang st, th)),
-        (P tid lang th):Prop).
+    (forall tid lang st th (TH: IdentMap.find tid (Threads.compose ths1 ths2) = Some (existT Language.state lang st, th)),
+        (P tid lang st th):Prop) <->
+    (forall tid lang st th (TH: IdentMap.find tid ths1 = Some (existT Language.state lang st, th)),
+        (P tid lang st th):Prop) /\
+    (forall tid lang st th (TH: IdentMap.find tid ths2 = Some (existT Language.state lang st, th)),
+        (P tid lang st th):Prop).
   Proof.
     econs; i.
-    - splits.
+    - i. splits.
       + i. eapply H; eauto.
         rewrite Threads.compose_spec. rewrite TH. ss.
       + i. eapply H; eauto.
@@ -56,21 +56,22 @@ Section Compose.
   Qed.
 
   Lemma compose_forall_rev P:
-    (forall tid lang st th (TH: IdentMap.find tid ths1 = Some (existT _ lang st, th)),
-        (P tid lang th):Prop) ->
-    (forall tid lang st th (TH: IdentMap.find tid ths2 = Some (existT _ lang st, th)),
-        (P tid lang th):Prop) ->
-    (forall tid lang st th (TH: IdentMap.find tid (Threads.compose ths1 ths2) = Some (existT _ lang st, th)),
-        (P tid lang th):Prop).
+    (forall tid lang st th (TH: IdentMap.find tid ths1 = Some (existT Language.state lang st, th)),
+        (P tid lang st th):Prop) ->
+    (forall tid lang st th (TH: IdentMap.find tid ths2 = Some (existT Language.state lang st, th)),
+        (P tid lang st th):Prop) ->
+    (forall tid lang st th (TH: IdentMap.find tid (Threads.compose ths1 ths2) = Some (existT Language.state lang st, th)),
+        (P tid lang st th):Prop).
   Proof.
-    i. eapply compose_forall; eauto.
-  Qed.    
+    i. apply compose_forall; auto.
+  Qed.
 
   Lemma compose_is_terminal:
     Threads.is_terminal (Threads.compose ths1 ths2) <->
     Threads.is_terminal ths1 /\ Threads.is_terminal ths2.
   Proof.
-    refine (compose_forall _). . ; eauto. Qed.
+    apply compose_forall.
+  Qed.
 
   Lemma compose_threads_consistent mem:
     Threads.consistent (Threads.compose ths1 ths2) mem <->
@@ -162,13 +163,13 @@ Proof.
   destruct (IdentMap.find tid ths1) eqn:TH1,
            (IdentMap.find tid ths2) eqn:TH2; inv TID.
   - exfalso. inv DISJOINT. eapply THREAD; eauto.
-  - left. exists (IdentMap.add tid (existT _ lang th3) ths1). splits; [|econs; eauto].
+  - left. exists (IdentMap.add tid (existT _ lang st3, th3) ths1). splits; [|econs; eauto].
     apply IdentMap.eq_leibniz. ii.
     rewrite ? IdentMap.Facts.add_o.
     rewrite ? Threads.compose_spec.
     rewrite ? IdentMap.Facts.add_o.
     destruct (IdentMap.Facts.eq_dec tid y); auto.
-  - right. exists (IdentMap.add tid (existT _ lang th3) ths2). splits; [|econs; eauto].
+  - right. exists (IdentMap.add tid (existT _ lang st3, th3) ths2). splits; [|econs; eauto].
     apply IdentMap.eq_leibniz. ii.
     rewrite ? IdentMap.Facts.add_o.
     rewrite ? Threads.compose_spec.
@@ -196,8 +197,8 @@ Lemma compose_step1
 Proof.
   exploit Configuration.step_disjoint; eauto. s. i. des.
   splits; eauto. inv STEP. ss.
-  replace (Threads.compose (IdentMap.add tid (existT _ lang th3) ths1) ths2)
-  with (IdentMap.add tid (existT _ lang th3) (Threads.compose ths1 ths2)).
+  replace (Threads.compose (IdentMap.add tid (existT _ lang st3, th3) ths1) ths2)
+  with (IdentMap.add tid (existT _ lang st3, th3) (Threads.compose ths1 ths2)).
   - econs; eauto.
     s. rewrite Threads.compose_spec. unfold Threads.compose_option.
     rewrite TID. auto.
