src/opt/ReorderWrite.v
@@ -1,0 +1,536 @@
+Require Import Basics.
+Require Import Bool.
+Require Import List.
+
+Require Import sflib.
+Require Import paco.
+Require Import respectful5.
+
+Require Import Basic.
+Require Import Event.
+Require Import Language.
+Require Import Time.
+Require Import Memory.
+Require Import Commit.
+Require Import Thread.
+
+Require Import Configuration.
+Require Import Simulation.
+Require Import Compatibility.
+Require Import MemInv.
+
+Require Import Syntax.
+Require Import Semantics.
+
+Set Implicit Arguments.
+
+Inductive sim_write (loc:Loc.t) (val:Const.t) (ord:Ordering.t) (th_src th_tgt:Local.t): Prop :=
+| sim_write_intro
+    commit2_src from to released
+    (COMMIT1: Commit.write th_src.(Local.commit) loc to released ord commit2_src)
+    (COMMIT2: Commit.le commit2_src th_tgt.(Local.commit))
+    (LT: Time.lt from to)
+    (PROMISE: MemInv.sem (Memory.singleton loc (Message.mk val released) LT) th_src.(Local.promise) th_tgt.(Local.promise))
+.
+
+Lemma sim_write_begin
+      loc val ord
+      th1_src mem1_src
+      th1_tgt mem1_tgt
+      th2_tgt mem2_tgt
+      (LOCAL1: sim_local th1_src th1_tgt)
+      (MEMORY1: sim_memory mem1_src mem1_tgt)
+      (WF1_SRC: Local.wf th1_src mem1_src)
+      (WF1_TGT: Local.wf th1_tgt mem1_tgt)
+      (STEP_TGT: Local.memory_step th1_tgt mem1_tgt (MemEvent.write loc val ord) th2_tgt mem2_tgt):
+  (<<LOCAL2: sim_write loc val ord th1_src th2_tgt>> /\
+   <<MEMORY2: sim_memory mem1_src mem2_tgt>>) \/
+  (exists th2_src mem2_src,
+      <<STEP_SRC: Local.promise_step th1_src mem1_src th2_src mem2_src>> /\
+      <<LOCAL2: sim_write loc val ord th2_src th2_tgt>> /\
+      <<MEMORY2: sim_memory mem2_src mem2_tgt>>).
+Proof.
+  inv STEP_TGT. inv MEMORY.
+  - left. splits; auto.
+    inversion LOCAL1. apply MemInv.sem_bot_inv in PROMISE.
+    destruct th1_src, th1_tgt. ss. subst.
+    inv CONFIRM.
+    econs; s.
+    + eapply CommitFacts.write_mon; eauto.
+    + reflexivity.
+    + econs. memtac.
+  - right. inv ADD.
+    exploit MemInv.promise; eauto.
+    { apply WF1_SRC. }
+    { apply WF1_TGT. }
+    { apply LOCAL1. }
+    i. des.
+    apply MemInv.sem_bot_inv in INV2. subst.
+    exploit Memory.promise_future; try apply PROMISE_SRC; eauto.
+    { apply WF1_SRC. }
+    { apply WF1_SRC. }
+    i. des.
+    eexists _, _. splits.
+    + econs; try apply PROMISE_SRC; eauto.
+      * reflexivity.
+      * eapply Commit.future_wf; eauto. apply WF1_SRC.
+    + inversion LOCAL1. apply MemInv.sem_bot_inv in PROMISE0.
+      destruct th1_src, th1_tgt. ss. subst.
+      inv CONFIRM.
+      econs; s.
+      * eapply CommitFacts.write_mon; eauto.
+      * reflexivity.
+      * econs. memtac.
+    + auto.
+Qed.
+
+Lemma sim_write_end
+      loc val ord
+      th1_src mem1_src
+      th1_tgt mem1_tgt
+      (ORD: Ordering.le ord Ordering.relaxed)
+      (LOCAL1: sim_write loc val ord th1_src th1_tgt)
+      (MEMORY1: sim_memory mem1_src mem1_tgt)
+      (WF1_SRC: Local.wf th1_src mem1_src)
+      (WF1_TGT: Local.wf th1_tgt mem1_tgt):
+  exists th2_src mem2_src,
+    <<STEP_SRC: Local.memory_step th1_src mem1_src (MemEvent.write loc val ord) th2_src mem2_src>> /\
+    <<LOCAL2: sim_local th2_src th1_tgt>> /\
+    <<MEMORY2: sim_memory mem2_src mem1_tgt>>.
+Proof.
+  destruct (Ordering.le Ordering.release ord) eqn:ORD2.
+  { destruct ord; ss. }
+  inv LOCAL1. inversion COMMIT1.
+  exploit Memory.le_get.
+  { apply WF1_SRC. }
+  { inv PROMISE. eapply Memory.le_get.
+    - apply Memory.le_join_r. memtac.
+    - apply Memory.singleton_get.
+  }
+  intro GET_SRC.
+  exploit CommitFacts.write_min_spec; eauto.
+  { instantiate (1 := ord). unfold CommitFacts.write_min.
+    rewrite ORD2. ss. etransitivity; [apply MONOTONE|apply RELEASED].
+  }
+  { apply WF1_SRC. }
+  { apply WF1_SRC. }
+  { inv WF1_SRC. inv MEMORY. exploit WF; eauto. }
+  i. des.
+  eexists _, _. splits; eauto.
+  - econs; eauto. econs 1.
+    + inv PROMISE. econs; ss.
+    + rewrite ORD2. ss.
+  - econs; ss.
+    + rewrite <- COMMIT2. eapply CommitFacts.write_min_min. eauto.
+    + apply MemInv.sem_bot.
+Qed.
+
+Lemma sim_local_promise
+      th1_src mem1_src
+      th1_tgt mem1_tgt
+      th2_tgt mem2_tgt
+      (LOCAL1: sim_local th1_src th1_tgt)
+      (MEMORY1: sim_memory mem1_src mem1_tgt)
+      (WF1_SRC: Local.wf th1_src mem1_src)
+      (WF1_TGT: Local.wf th1_tgt mem1_tgt)
+      (STEP_TGT: Local.promise_step th1_tgt mem1_tgt th2_tgt mem2_tgt):
+  exists th2_src mem2_src,
+    <<STEP_SRC: Local.promise_step th1_src mem1_src th2_src mem2_src>> /\
+    <<LOCAL2: sim_local th2_src th2_tgt>> /\
+    <<MEMORY2: sim_memory mem2_src mem2_tgt>>.
+Proof.
+  inv LOCAL1. inv STEP_TGT.
+  exploit MemInv.promise; eauto.
+  { apply WF1_SRC. }
+  { apply WF1_TGT. }
+  i. des.
+  exploit Memory.promise_future; try apply PROMISE_SRC; eauto.
+  { apply WF1_SRC. }
+  { apply WF1_SRC. }
+  i. des.
+  eexists _, _. splits; eauto.
+  - econs; try apply PROMISE_SRC.
+    + reflexivity.
+    + eapply Commit.future_wf; [|eauto]. apply WF1_SRC.
+  - econs; s; eauto. etransitivity; eauto.
+Qed.
+
+Lemma sim_write_promise
+      loc val ord
+      th1_src mem1_src
+      th1_tgt mem1_tgt
+      th2_tgt mem2_tgt
+      (ORD: Ordering.le ord Ordering.relaxed)
+      (LOCAL1: sim_write loc val ord th1_src th1_tgt)
+      (MEMORY1: sim_memory mem1_src mem1_tgt)
+      (WF1_SRC: Local.wf th1_src mem1_src)
+      (WF1_TGT: Local.wf th1_tgt mem1_tgt)
+      (STEP_TGT: Local.promise_step th1_tgt mem1_tgt th2_tgt mem2_tgt):
+  exists th2_src mem2_src,
+    <<STEP_SRC: Local.promise_step th1_src mem1_src th2_src mem2_src>> /\
+    <<LOCAL2: sim_write loc val ord th2_src th2_tgt>> /\
+    <<MEMORY2: sim_memory mem2_src mem2_tgt>>.
+Proof.
+  inv LOCAL1. inv STEP_TGT.
+  exploit MemInv.promise; eauto.
+  { apply WF1_SRC. }
+  { apply WF1_TGT. }
+  i. des.
+  exploit Memory.promise_future; try apply PROMISE_SRC; eauto.
+  { apply WF1_SRC. }
+  { apply WF1_SRC. }
+  i. des.
+  eexists _, _. splits; eauto.
+  - econs; eauto.
+    + reflexivity.
+    + eapply Commit.future_wf; eauto. apply WF1_SRC.
+  - econs; s; eauto. etransitivity; eauto.
+Qed.
+
+Lemma sim_write_read
+      loc1 val1 ord1
+      loc2 val2 ord2
+      th1_src mem1_src
+      th1_tgt mem1_tgt
+      th2_tgt mem2_tgt
+      (LOC: loc1 <> loc2)
+      (ORD1: Ordering.le ord1 Ordering.relaxed)
+      (ORD2: Ordering.le ord2 Ordering.relaxed)
+      (LOCAL1: sim_write loc1 val1 ord1 th1_src th1_tgt)
+      (MEMORY1: sim_memory mem1_src mem1_tgt)
+      (WF1_SRC: Local.wf th1_src mem1_src)
+      (WF1_TGT: Local.wf th1_tgt mem1_tgt)
+      (STEP_TGT: Local.memory_step th1_tgt mem1_tgt (MemEvent.read loc2 val2 ord2) th2_tgt mem2_tgt):
+  exists th2_src mem2_src,
+    <<STEP_SRC: Local.memory_step th1_src mem1_src (MemEvent.read loc2 val2 ord2) th2_src mem2_src>> /\
+    <<LOCAL2: sim_write loc1 val1 ord1 th2_src th2_tgt>> /\
+    <<MEMORY2: sim_memory mem2_src mem2_tgt>>.
+Proof.
+  inv LOCAL1. inv STEP_TGT.
+  exploit Memory.le_get.
+  { apply WF1_SRC. }
+  { inv PROMISE. eapply Memory.le_get.
+    - apply Memory.le_join_r. memtac.
+    - apply Memory.singleton_get.
+  }
+  intro GET1_SRC.
+  exploit Memory.splits_get; try apply GET; eauto.
+  { inv MEMORY1. eauto. }
+  intro GET2_SRC.
+  exploit CommitFacts.read_min_spec; try apply GET2_SRC; eauto.
+  { inv COMMIT. eapply Snapshot.readable_mon; eauto.
+    etransitivity; [|apply COMMIT2]. apply COMMIT1.
+  }
+  { apply WF1_SRC. }
+  { apply WF1_SRC. }
+  i. des.
+  destruct (Ordering.le Ordering.release ord1) eqn:ORD1'.
+  { destruct ord1; ss. }
+  assert (RELEASED_SRC: Memory.wf_snapshot released mem1_src).
+  { inv WF1_SRC. inv MEMORY. exploit WF0; try apply GET1_SRC; eauto. }
+  exploit CommitFacts.write_min_spec; try apply RELEASED_SRC; eauto.
+  { eapply Snapshot.le_on_writable; eauto. apply COMMIT1. }
+  { instantiate (1 := ord1).
+    unfold CommitFacts.write_min. rewrite ORD1'. ss.
+    inv COMMIT1. etransitivity; [apply MONOTONE|apply RELEASED].
+  }
+  { apply WF1_SRC. }
+  i. des.
+  eexists _, _. splits; eauto.
+  - econs; eauto. inv PROMISE.
+    match goal with
+    | [|- ?x = None] => destruct x eqn:X; auto
+    end.
+    apply Memory.join_get in X; memtac; try congruence.
+    apply Memory.singleton_get_inv in X. des. congruence.
+  - econs; s; eauto.
+    exploit CommitFacts.write_min_min; try apply COMMIT1; eauto. i.
+    exploit CommitFacts.read_min_min; try apply COMMIT; eauto. i.
+    inv x0. inv x1. inv CURRENT1. inv CURRENT2. econs.
+    + econs; ss.
+      * etransitivity; [|eauto].
+        apply Times.incr_mon. etransitivity; [|apply COMMIT2]. apply COMMIT1.
+      * etransitivity; eauto. etransitivity; eauto. apply COMMIT2.
+    + i. etransitivity; eauto.
+      unfold CommitFacts.write_min. rewrite ORD1'. ss.
+      etransitivity; eauto; [|apply COMMIT2]. apply COMMIT1.
+    + etransitivity; eauto.
+      apply Snapshot.join_spec.
+      * apply Snapshot.join_l.
+      * etransitivity; [|apply Snapshot.join_r].
+        etransitivity; [|apply COMMIT2]. apply COMMIT1.
+Qed.
+
+Lemma sim_write_write
+      loc1 val1 ord1
+      loc2 val2 ord2
+      th1_src mem1_src
+      th1_tgt mem1_tgt
+      th2_tgt mem2_tgt
+      (LOC: loc1 <> loc2)
+      (ORD1: Ordering.le ord1 Ordering.relaxed)
+      (LOCAL1: sim_write loc1 val1 ord1 th1_src th1_tgt)
+      (MEMORY1: sim_memory mem1_src mem1_tgt)
+      (WF1_SRC: Local.wf th1_src mem1_src)
+      (WF1_TGT: Local.wf th1_tgt mem1_tgt)
+      (STEP_TGT: Local.memory_step th1_tgt mem1_tgt (MemEvent.write loc2 val2 ord2) th2_tgt mem2_tgt):
+  exists th2_src mem2_src,
+    <<STEP_SRC: Local.memory_step th1_src mem1_src (MemEvent.write loc2 val2 ord2) th2_src mem2_src>> /\
+    <<LOCAL2: sim_write loc1 val1 ord1 th2_src th2_tgt>> /\
+    <<MEMORY2: sim_memory mem2_src mem2_tgt>>.
+Proof.
+Admitted.
+
+Lemma sim_write_update
+      loc1 val1 ord1
+      loc2 val21 val22 ord2
+      th1_src mem1_src
+      th1_tgt mem1_tgt
+      th2_tgt mem2_tgt
+      (LOC: loc1 <> loc2)
+      (ORD1: Ordering.le ord1 Ordering.relaxed)
+      (ORD2: Ordering.le ord2 Ordering.release)
+      (LOCAL1: sim_write loc1 val1 ord1 th1_src th1_tgt)
+      (MEMORY1: sim_memory mem1_src mem1_tgt)
+      (WF1_SRC: Local.wf th1_src mem1_src)
+      (WF1_TGT: Local.wf th1_tgt mem1_tgt)
+      (STEP_TGT: Local.memory_step th1_tgt mem1_tgt (MemEvent.update loc2 val21 val22 ord2) th2_tgt mem2_tgt):
+  exists th2_src mem2_src,
+    <<STEP_SRC: Local.memory_step th1_src mem1_src (MemEvent.update loc2 val21 val22 ord2) th2_src mem2_src>> /\
+    <<LOCAL2: sim_write loc1 val1 ord1 th2_src th2_tgt>> /\
+    <<MEMORY2: sim_memory mem2_src mem2_tgt>>.
+Proof.
+Admitted.
+
+Inductive reorder l2 v2 o2: forall (i1:Instr.t), Prop :=
+| reorder_load
+    r1 l1 o1
+    (ORD1: Ordering.le o1 Ordering.relaxed)
+    (ORD2: Ordering.le o2 Ordering.relaxed)
+    (LOC: l2 <> l1)
+    (DISJOINT: RegSet.disjoint (Instr.regs_of (Instr.load r1 l1 o1))
+                               (Instr.regs_of (Instr.store l2 v2 o2))):
+    reorder l2 v2 o2 (Instr.load r1 l1 o1)
+| reorder_store
+    l1 v1 o1
+    (ORD2: Ordering.le o2 Ordering.relaxed)
+    (LOC: l2 <> l1)
+    (DISJOINT: RegSet.disjoint (Instr.regs_of (Instr.store l1 v1 o1))
+                               (Instr.regs_of (Instr.store l2 v2 o2))):
+    reorder l2 v2 o2 (Instr.store l1 v1 o1)
+| reorder_update
+    r1 l1 rmw1 o1
+    (ORD1: Ordering.le o1 Ordering.release)
+    (ORD2: Ordering.le o2 Ordering.relaxed)
+    (LOC: l2 <> l1)
+    (DISJOINT: RegSet.disjoint (Instr.regs_of (Instr.update r1 l1 rmw1 o1))
+                               (Instr.regs_of (Instr.store l2 v2 o2))):
+    reorder l2 v2 o2 (Instr.update r1 l1 rmw1 o1)
+.
+
+Inductive sim: forall (st_src:lang.(Language.state)) (th_src:Local.t) (mem_k_src:Memory.t)
+                 (st_tgt:lang.(Language.state)) (th_tgt:Local.t) (mem_k_tgt:Memory.t), Prop :=
+| sim_begin
+    i1 l2 v2 o2
+    rs th_src th_tgt
+    mem_k_src mem_k_tgt
+    (REORDER: reorder l2 v2 o2 i1)
+    (LOCAL: sim_local th_src th_tgt):
+    sim
+      (State.mk rs [Stmt.instr Instr.skip; Stmt.instr i1; Stmt.instr (Instr.store l2 v2 o2)]) th_src mem_k_src
+      (State.mk rs [Stmt.instr (Instr.store l2 v2 o2); Stmt.instr i1]) th_tgt mem_k_tgt
+| sim_end
+    rs th_src th_tgt
+    mem_k_src mem_k_tgt
+    (LOCAL: sim_local th_src th_tgt):
+    sim
+      (State.mk rs []) th_src mem_k_src
+      (State.mk rs []) th_tgt mem_k_tgt
+| sim_intermediate
+    i1 l2 v2 o2
+    rs th_src th_tgt
+    mem_k_src mem_k_tgt
+    (REORDER: reorder l2 v2 o2 i1)
+    (LOCAL: sim_write l2 (RegFile.eval_value rs v2) o2 th_src th_tgt):
+    sim
+      (State.mk rs [Stmt.instr i1; Stmt.instr (Instr.store l2 v2 o2)]) th_src mem_k_src
+      (State.mk rs [Stmt.instr i1]) th_tgt mem_k_tgt
+.
+
+Lemma Memory_write_bot
+      mem1 loc from to msg ord promise2 mem2
+      (WRITE: Memory.write Memory.bot mem1 loc from to msg ord promise2 mem2):
+  promise2 = Memory.bot.
+Proof.
+Admitted.
+
+Lemma sim_reorder_sim_stmts:
+  sim <6= (sim_thread (sim_terminal eq)).
+Proof.
+  pcofix CIH. i. pfold. ii. ss. splits; ss.
+  - i. inv TERMINAL_TGT. inv PR; ss.
+    eexists _, _, _. splits; eauto. econs; ss.
+  - admit.
+    (* future; https://github.com/jeehoonkang/memory-model-explorer/blob/86c803103989f87a17f50e6349aa9f285104af09/formalization/src/opt/Reorder.v#L100 *)
+  - i. inv PR.
+    + inv LOCAL. apply MemInv.sem_bot_inv in PROMISE.
+      eexists _, _, _. splits; eauto. etransitivity; eauto.
+    + inv LOCAL. apply MemInv.sem_bot_inv in PROMISE.
+      eexists _, _, _. splits; eauto. etransitivity; eauto.
+    + inv REORDER.
+      * assert (STEP: exists val th2_tgt mem2_tgt,
+                   Local.memory_step x4 mem1_tgt (MemEvent.read l1 val o1) th2_tgt mem2_tgt).
+        { admit.
+          (* https://github.com/jeehoonkang/memory-model-explorer/blob/86c803103989f87a17f50e6349aa9f285104af09/formalization/src/opt/Reorder.v#L116 *)
+        }
+        des.
+        exploit sim_write_read; try apply LOCAL; try apply STEP; eauto. i. des.
+        exploit sim_write_end; eauto.
+        { eapply Local.memory_step_future; eauto. }
+        { eapply Local.memory_step_future; eauto. }
+        i. des.
+        eexists _, _, _. splits.
+        { econs 2; [|econs 2; [|econs 1]].
+          - econs 3; eauto. econs. econs.
+          - econs 3; eauto. econs.
+            erewrite <- RegFile.eq_except_value; eauto.
+            + econs.
+            + apply RegFile.eq_except_singleton.
+        }
+        inv LOCAL0. apply MemInv.sem_bot_inv in PROMISE.
+        etransitivity; eauto.
+        inv STEP. ss.
+      * assert (STEP: exists th2_tgt mem2_tgt,
+                   Local.memory_step x4 mem1_tgt (MemEvent.write l1 (RegFile.eval_value rs v1) o1) th2_tgt mem2_tgt).
+        { admit. }
+        des.
+        exploit sim_write_write; try apply LOCAL; try apply STEP; eauto. i. des.
+        exploit sim_write_end; eauto.
+        { eapply Local.memory_step_future; eauto. }
+        { eapply Local.memory_step_future; eauto. }
+        i. des.
+        eexists _, _, _. splits.
+        { econs 2; [|econs 2; [|econs 1]].
+          - econs 3; eauto. econs. econs.
+          - econs 3; eauto. econs. econs.
+        }
+        inv LOCAL0. apply MemInv.sem_bot_inv in PROMISE.
+        etransitivity; eauto.
+        inv STEP. ss.
+        rewrite PROMISE_TGT in *. eapply Memory_write_bot. eauto.
+      * assert (STEP: exists old new th2_tgt mem2_tgt,
+           <<STEP: Local.memory_step x4 mem1_tgt (MemEvent.update l1 old new o1) th2_tgt mem2_tgt>> /\
+           <<RMW: RegFile.eval_rmw rs rmw1 old new>>).
+        { admit. }
+        des.
+        exploit sim_write_update; try apply LOCAL; try apply STEP0; eauto. i. des.
+        exploit sim_write_end; eauto.
+        { eapply Local.memory_step_future; eauto. }
+        { eapply Local.memory_step_future; eauto. }
+        i. des.
+        eexists _, _, _. splits.
+        { econs 2; [|econs 2; [|econs 1]].
+          - econs 3; eauto. econs. econs. auto.
+          - econs 3; eauto. econs.
+            erewrite <- RegFile.eq_except_value; eauto.
+            + econs.
+            + admit. (* regfile disjoint *)
+        }
+        inv LOCAL0. apply MemInv.sem_bot_inv in PROMISE.
+        etransitivity; eauto.
+        inv STEP0. ss.
+        rewrite PROMISE_TGT in *. eapply Memory_write_bot. eauto.
+  - i. inv PR; ss.
+    + (* begin *)
+      inv STEP_TGT; inv STEP; try (inv STATE; inv INSTR); ss.
+      * exploit sim_local_promise; eauto. i. des.
+        eexists _, _, _, _, _, _. splits; eauto.
+        { econs. econs 1. eauto. }
+        right. apply CIH. econs 1; ss.
+      * exploit sim_write_begin; eauto. i. des.
+        { eexists _, _, _, _, _, _. splits; try apply MEMORY2; eauto.
+          { econs. econs 3; ss.
+            - econs. econs.
+            - apply Local.fence_relaxed. ss.
+          }
+          right. apply CIH. econs 3; eauto.
+        }
+        { eexists _, _, _, _, _, _. splits; try apply MEMORY2.
+          { econs 2; [|econs 1].
+            econs 3; ss.
+            - econs. econs.
+            - apply Local.fence_relaxed. ss.
+          }
+          { econs. econs 1; eauto. }
+          right. apply CIH. econs 3; eauto.
+        }
+    + (* end *)
+      inv STEP_TGT; inv STEP; try (inv STATE; inv INSTR); ss.
+      exploit sim_local_promise; eauto. i. des.
+      eexists _, _, _, _, _, _. splits; eauto.
+      { econs. econs 1. eauto. }
+      right. apply CIH. econs 2; ss.
+    + (* intermediate *)
+      inv STEP_TGT; inv STEP; try (inv STATE; inv INSTR; inversion REORDER); subst; ss.
+      * exploit sim_write_promise; eauto.
+        { inv REORDER; ss. }
+        i. des.
+        eexists _, _, _, _, _, _. splits; eauto.
+        { econs. econs 1. eauto. }
+        right. apply CIH. econs 3; ss.
+      * exploit sim_write_read; try apply LOCAL; try apply STEP0; eauto. i. des.
+        exploit sim_write_end; eauto.
+        { eapply Local.memory_step_future; eauto. }
+        { eapply Local.memory_step_future; eauto. }
+        i. des.
+        eexists _, _, _, _, _, _. splits.
+        { econs 2; [|econs 1].
+          econs 3; eauto. econs. econs.
+        }
+        { econs. econs 3; eauto. econs.
+          erewrite <- RegFile.eq_except_value; eauto.
+          - econs.
+          - apply RegFile.eq_except_singleton.
+        }
+        { eauto. }
+        right. apply CIH. econs 2; eauto.
+      * exploit sim_write_write; try apply LOCAL; try apply STEP; eauto. i. des.
+        exploit sim_write_end; eauto.
+        { eapply Local.memory_step_future; eauto. }
+        { eapply Local.memory_step_future; eauto. }
+        i. des.
+        eexists _, _, _, _, _, _. splits.
+        { econs 2; [|econs 1].
+          econs 3; eauto. econs. econs.
+        }
+        { econs. econs 3; eauto. econs. econs. }
+        { eauto. }
+        right. apply CIH. econs 2; eauto.
+      * exploit sim_write_update; try apply LOCAL; try apply STEP0; eauto. i. des.
+        exploit sim_write_end; eauto.
+        { eapply Local.memory_step_future; eauto. }
+        { eapply Local.memory_step_future; eauto. }
+        i. des.
+        eexists _, _, _, _, _, _. splits.
+        { econs 2; [|econs 1].
+          econs 3; eauto. econs. econs. auto.
+        }
+        { econs. econs 3; eauto. econs.
+          erewrite <- RegFile.eq_except_value; eauto.
+          - econs.
+          - admit. (* regfile disjoint *)
+        }
+        { eauto. }
+        right. apply CIH. econs 2; eauto.
+Admitted.
+
+Lemma reorder_sim_stmts
+      i1 l2 v2 o2 (REORDER: reorder l2 v2 o2 i1):
+  sim_stmts eq
+            [Stmt.instr Instr.skip; Stmt.instr i1; Stmt.instr (Instr.store l2 v2 o2)]
+            [Stmt.instr (Instr.store l2 v2 o2); Stmt.instr i1]
+            eq.
+Proof.
+  ii. subst.
+  eapply sim_reorder_sim_stmts; eauto. econs 1; auto.
+Qed.
